Fill in for admits

src/specs/UpdateAggregationChallenge.ec
@@ -1,10 +1,15 @@
+pragma Goals:printall.
+
 require        Constants.
 require import PointMulAndAddIntoDest.
 require import PurePrimops.
 require import UInt256.
+require import Utils.
 require import Verifier.
 require import VerifierConsts.
 require import YulPrimops.
+
+import MemoryMap.
 
 module UpdateAggregationChallenge = {
   proc low(queriesCommitmentPoint : uint256, valueAtZ : uint256, curAggregationChallenge : uint256, curAggregatedOpeningAtZ : uint256): (uint256 * uint256) = {
@@ -32,25 +37,6 @@ module UpdateAggregationChallenge = {
   }
 }.
 
-op UpdateAggregationChallenge_footprint (x y x' y' : F) (currAggregatedAtZXSlot : int * int) (memory0 : MemoryMap.mem) =
-           (PurePrimops.mstore
-              ((PurePrimops.mstore
-                  ((PurePrimops.mstore
-                      ((PurePrimops.mstore
-                          ((PurePrimops.mstore
-                              (PurePrimops.mstore memory0 W256.zero
-                                  ((of_int (ZModField.asint x)))%W256)
-                              ((of_int 32))%W256
-                              ((of_int (ZModField.asint y)))%W256))
-                          ((of_int 64))%W256
-                          ((W256.of_int currAggregatedAtZXSlot.`1))%W256))%PurePrimops
-                      ((of_int 96))%W256
-                      ((of_int currAggregatedAtZXSlot.`2))%W256))%PurePrimops
-                  AGGREGATED_AT_Z_X_SLOT
-                  ((of_int (ZModField.asint x')))%W256))%PurePrimops
-              (AGGREGATED_AT_Z_X_SLOT + (of_int 32)%W256)
-              ((of_int (ZModField.asint y')%ZModField))%W256)%PurePrimops.
-
 lemma UpdateAggregationChallenge_extracted_equiv_low :
     equiv [
       Verifier_1261.usr_updateAggregationChallenge ~ UpdateAggregationChallenge.low :
@@ -63,6 +49,59 @@ proof.
   call (pointMulAndAddIntoDest_extracted_equiv_low). wp.
   skip. rewrite /Constants.R. by progress.
 qed.
+
+
+op UpdateAggregationChallenge_footprint (x y x' y' : int) (currAggregatedAtZXSlot : int * int) (mem_0 : mem) =
+  let mem_1 = store mem_0 W256.zero (W256.of_int x) in
+  let mem_2 = store mem_1 (W256.of_int 32) (W256.of_int y) in
+  let mem_3 = store mem_2 (W256.of_int 64) (W256.of_int currAggregatedAtZXSlot.`1) in
+  let mem_4 = store mem_3 (W256.of_int 96) (W256.of_int currAggregatedAtZXSlot.`2) in
+  let mem_5 = store mem_4 AGGREGATED_AT_Z_X_SLOT (W256.of_int x') in
+  store mem_5 AGGREGATED_AT_Z_Y_SLOT (W256.of_int y').
+
+
+(* smt cannot prove these in the proof because there's too many assumptions in play *)
+lemma diff_96 (a: uint256): W256.of_int 128 <= a => W256.of_int 32 <= a - W256.of_int 96.
+    proof.
+      progress.
+      smt (@W256 @Utils).
+  qed.
+lemma diff_64 (a: uint256): W256.of_int 128 <= a => W256.of_int 32 <= a - W256.of_int 64.
+    proof.
+      progress.
+      smt (@W256 @Utils).
+  qed.
+lemma diff_32 (a: uint256): W256.of_int 128 <= a => W256.of_int 32 <= a - W256.of_int 32.
+    proof.
+      progress.
+      smt (@W256 @Utils).
+  qed.
+lemma diff_0 (a: uint256): W256.of_int 128 <= a => W256.of_int 32 <= a - W256.zero.
+    proof.
+      progress.
+      smt (@W256 @Utils).
+  qed.
+lemma diff_neg_96 (a: uint256): W256.of_int 128 <= a => W256.of_int 32 <= -a => W256.of_int 32 <= W256.of_int 96 - a.
+    proof.
+      progress.
+    smt (@W256 @Utils).
+  qed.
+lemma diff_neg_64 (a: uint256): W256.of_int 128 <= a => W256.of_int 32 <= -a => W256.of_int 32 <= W256.of_int 64 - a.
+    proof.
+      progress.
+    smt (@W256 @Utils).
+  qed.  
+lemma diff_neg_32 (a: uint256): W256.of_int 128 <= a => W256.of_int 32 <= -a => W256.of_int 32 <= W256.of_int 32 - a.
+    proof.
+      progress.
+    smt (@W256 @Utils).
+  qed.
+lemma diff_neg_0 (a: uint256): W256.of_int 128 <= a => W256.of_int 32 <= -a => W256.of_int 32 <= W256.zero - a.
+    proof.
+      progress.
+  qed.
+
+   
 
 lemma UpdateAggregationChallenge_mid_of_low (queriesCommitmentPoint : int * int) (currAggregatedAtZXSlot : int * int) (valueAtZ : int) (currAggregationChallenge : int) (curAggregatedOpeningAtZ : int) (v_challenge : int) (queriesCommitmentPoint_addr valueAtZ_addr : uint256) (memory0 : MemoryMap.mem) : equiv [
     UpdateAggregationChallenge.low ~ UpdateAggregationChallenge.mid :
@@ -79,6 +118,12 @@ lemma UpdateAggregationChallenge_mid_of_low (queriesCommitmentPoint : int * int)
     W256.of_int 64 <= - queriesCommitmentPoint_addr /\
     W256.of_int 128 <= queriesCommitmentPoint_addr + W256.of_int 32 /\
     W256.of_int 32 <= - (queriesCommitmentPoint_addr + W256.of_int 32) /\
+    W256.of_int 128 <= valueAtZ_addr /\
+    W256.of_int 32 <= -valueAtZ_addr /\
+    W256.of_int 32 <= valueAtZ_addr - (AGGREGATED_AT_Z_X_SLOT + W256.of_int 32) /\
+    W256.of_int 32 <= AGGREGATED_AT_Z_X_SLOT - valueAtZ_addr /\
+    W256.of_int 32 <= valueAtZ_addr - AGGREGATED_AT_Z_X_SLOT /\
+    W256.of_int 32 <= (AGGREGATED_AT_Z_X_SLOT + W256.of_int 32) - valueAtZ_addr /\
     arg{1} = (queriesCommitmentPoint_addr, valueAtZ_addr, W256.of_int currAggregationChallenge, W256.of_int curAggregatedOpeningAtZ) /\
     arg{2} = (queriesCommitmentPoint, currAggregatedAtZXSlot, valueAtZ, currAggregationChallenge, curAggregatedOpeningAtZ, v_challenge) /\
     PurePrimops.mload memory0 STATE_V_SLOT = W256.of_int v_challenge /\
@@ -92,16 +137,12 @@ lemma UpdateAggregationChallenge_mid_of_low (queriesCommitmentPoint : int * int)
       (res{2} = None /\ Primops.reverted{1}) \/
       (
         exists (newAggregationChallenge newAggregatedOpeningAtZ : int) (newAggregateAtZXSlot : int * int),
-        (* newAggregationChallenge = v_challenge * currAggregationChallenge %% Constants.R /\ *)
-        (* newAggregatedOpeningAtZ = (v_challenge * currAggregationChallenge * valueAtZ + curAggregatedOpeningAtZ) %% Constants.R /\ *)
         res{2} = Some (newAggregationChallenge, newAggregatedOpeningAtZ, newAggregateAtZXSlot) /\
         res{1} = (W256.of_int newAggregationChallenge, W256.of_int newAggregatedOpeningAtZ) /\
-        (* Primops.memory{1} = UpdateAggregationChallenge_footprint queriesCommitmentPoint{2}.`1 queriesCommitmentPoint{2}.`2 /\ *)
-        Primops.memory{1} = PurePrimops.mstore (PurePrimops.mstore memory0 AGGREGATED_AT_Z_X_SLOT (W256.of_int newAggregateAtZXSlot.`1)) (AGGREGATED_AT_Z_X_SLOT + W256.of_int 32) (W256.of_int newAggregateAtZXSlot.`2) /\
+        (exists (x y: int),
+        Primops.memory{1} = UpdateAggregationChallenge_footprint x y newAggregateAtZXSlot.`1 newAggregateAtZXSlot.`2 currAggregatedAtZXSlot memory0) /\
         ! Primops.reverted{1}
-      )
-    
-      
+      )   
     ]. proof.
         proc. inline mload. wp. sp.
 
@@ -122,7 +163,7 @@ lemma UpdateAggregationChallenge_mid_of_low (queriesCommitmentPoint : int * int)
         rewrite of_uintK.
         smt ().
     
-        rewrite H19 /PurePrimops.mulmod.
+        rewrite H25 /PurePrimops.mulmod.
         simplify.
         rewrite of_uintK.
         have ->: to_uint R_MOD = Constants.R. smt (@Constants).
@@ -134,23 +175,32 @@ lemma UpdateAggregationChallenge_mid_of_low (queriesCommitmentPoint : int * int)
         exists ((v_challenge{2} * currAggregationChallenge{2} %% Constants.R * valueAtZ{2} + curAggregatedOpeningAtZ{2}) %% Constants.R).
         exists (odflt (0, 0) result_R).
         progress.
-        rewrite H19.
-        have ->: PurePrimops.mload memory_L valueAtZ{1} = W256.of_int valueAtZ{2}. admit.
-        rewrite /PurePrimops.addmod /PurePrimops.mulmod.
-        simplify.
-        rewrite /PurePrimops.mulmod. simplify.
-        rewrite of_uintK of_uintK of_uintK of_uintK of_uintK of_uintK of_uintK.
+        rewrite H25.
+        case H56; first last. progress. smt ().
+        progress. case H58; first last. progress. smt ().
+        progress.
+        rewrite load_store_diff. assumption. assumption.
+        rewrite load_store_diff. assumption. assumption.
+        rewrite load_store_diff. exact diff_96. exact diff_neg_96.
+        rewrite load_store_diff. exact diff_64. exact diff_neg_64.
+        rewrite load_store_diff. exact diff_32. exact diff_neg_32.
+        rewrite load_store_diff. exact diff_0. exact diff_neg_0.
+        rewrite H26. rewrite /addmod /mulmod. simplify. rewrite - Constants.R_int.
+        do rewrite W256.of_uintK.
         have ->: curAggregatedOpeningAtZ{2} %% W256.modulus = curAggregatedOpeningAtZ{2}. smt ().
         have ->: currAggregationChallenge{2} %% W256.modulus = currAggregationChallenge{2}. smt ().
         have ->: (v_challenge{2} %% W256.modulus) = v_challenge{2}. smt ().
         have ->: (valueAtZ{2} %% W256.modulus) = valueAtZ{2}. smt ().
-        have ->: (21888242871839275222246405745257275088548364400416034343698204186575808495617 %%
-        W256.modulus) = Constants.R. smt ().
+        rewrite (pmod_small _ W256.modulus). smt (@Constants @IntDiv).
+        rewrite (pmod_small _ W256.modulus). smt (@Constants @IntDiv).
         congr.
-        rewrite Utils.mod_mod_eq_mod. smt (). smt ().
-        rewrite Utils.mod_mod_eq_mod. smt (). smt ().
+        smt (@IntDiv).
+        case H56; first last. progress. smt ().
+        progress. case H58; first last. progress. smt ().
+        progress. rewrite /UpdateAggregationChallenge_footprint. simplify.
+        exists (ZModField.asint x). exists (ZModField.asint y). reflexivity.
         smt ().
-        admit. smt (). smt ().
+        smt ().
     qed.
     
 
